Pool: positivity annotations (FIXME, need to admit)

share/pulse/examples/NuPool.fst
@@ -196,14 +196,17 @@ let lock_inv (#code:vcode)
     BAR.pts_to_full g_runnable v_runnable **
     all_state_pred v_runnable
 
+#push-options "--__no_positivity"
 noeq
-type pool_st (code_t:Type u#2) : Type u#0 = {
+type pool_st ([@@@strictly_positive] code_t:Type u#2) : Type u#0 = {
   runnable   : Big.ref (list (task_t code_t));
   g_runnable : BAR.ref (list (task_t code_t)) list_preorder list_anchor;
   
   lk : lock; // (lock_inv runnable g_runnable);
 }
-type pool (code_t:Type u#2) : Type0 = pool_st code_t
+
+type pool ([@@@strictly_positive] code_t:Type u#2) : Type0 = pool_st code_t
+#pop-options
 
 let pool_alive (#[exact (`full_perm)] f : perm) (code:vcode) (p:pool code.t) : vprop =
   lock_alive p.lk #(half_perm f) (lock_inv p.runnable p.g_runnable)
